SSL-Cog/eyerok-manipulation/pipeline/prepare-sources.sh
@@ -23,9 +23,13 @@ extract src/engine/surface_collision.c surface_collision.c
 extract levels/ssl/script.c ssl_script.c
 extract src/game/area.c area.c
 extract src/game/level_update.c level_update.c
+extract src/game/game_init.c game_init.c
 extract src/game/mario.c mario.c
 extract src/game/mario_step.c mario_step.c
 extract src/game/mario_actions_airborne.c mario_actions_airborne.c
+extract src/game/mario_actions_moving.c mario_actions_moving.c
+extract src/game/mario_actions_object.c mario_actions_object.c
+extract src/game/mario_actions_stationary.c mario_actions_stationary.c
 extract src/game/platform_displacement.c platform_displacement.c
 extract src/game/interaction.c interaction.c
 
